cfrontend/Cminorgenproof.v
@@ -199,7 +199,7 @@ Record match_env (f: meminj) (cenv: compilenv)
   mk_match_env {
 
     me_sps:
-      sp = fresh_block true sps;
+      sp = fresh_block sps;
 
     me_sup_include:
       Mem.sup_include bes es;
@@ -291,7 +291,7 @@ Qed.
 Lemma match_env_alloc:
   forall f1 id cenv e sp sps bes m1 sz m2 b ofs f2,
   match_env f1 (PTree.remove id cenv) e sp sps bes (Mem.support m1) ->
-  Mem.alloc true m1 0 sz = (m2, b) ->
+  Mem.alloc m1 0 sz = (m2, b) ->
   cenv!id = Some ofs ->
   inject_incr f1 f2 ->
   f2 b = Some(sp, ofs) ->
@@ -324,7 +324,7 @@ Proof.
   exploit me_bounded0; eauto. rewrite SUPPORT. intros [A B].
   split. apply Mem.sup_incr_in2. auto. auto.
 (* inv *)
-  intros. destruct (eq_block b (Mem.nextblock true m1)).
+  intros. destruct (eq_block b (Mem.nextblock m1)).
   subst b. rewrite SAME in H; inv H. exists id; exists sz. apply PTree.gss.
   rewrite OTHER in H; auto. exploit me_inv0; eauto.
   intros [id1 [sz1 EQ]]. exists id1; exists sz1. rewrite PTree.gso; auto. congruence.
@@ -480,7 +480,7 @@ Inductive match_callstack (f: meminj) (m: mem) (tm: mem):
   | mcs_cons:
       forall cenv tf e le te sp sps bes es cs bound tbound
         (BOUND: Mem.sup_include es bound)
-        (TBOUND: Mem.sup_include (sup_incr true sps) tbound)
+        (TBOUND: Mem.sup_include (sup_incr sps) tbound)
         (MTMP: match_temps f le te)
         (MENV: match_env f cenv e sp sps bes es)
         (BOUND: match_bounds e m)
@@ -592,7 +592,7 @@ Lemma match_callstack_freelist:
   /\ Mem.inject f m' tm'.
 Proof.
   intros until tm; intros INJ FREELIST MCS. inv MCS. inv MENV.
-  assert ({tm' | Mem.free tm (fresh_block true sps) 0 (fn_stackspace tf) = Some tm'}).
+  assert ({tm' | Mem.free tm (fresh_block sps) 0 (fn_stackspace tf) = Some tm'}).
   apply Mem.range_perm_free.
   red; intros.
   exploit PERM; eauto. intros [A | A].
@@ -689,7 +689,7 @@ Qed.
 Lemma match_callstack_alloc_right:
   forall f m tm cs tf tm' sp le te cenv,
   match_callstack f m tm cs (Mem.support m) (Mem.support tm) ->
-  Mem.alloc true tm 0 tf.(fn_stackspace) = (tm', sp) ->
+  Mem.alloc tm 0 tf.(fn_stackspace) = (tm', sp) ->
   Mem.inject f m tm ->
   match_temps f le te ->
   (forall id, cenv!id = None) ->
@@ -718,11 +718,11 @@ Qed.
 
 Lemma match_callstack_alloc_left:
   forall f1 m1 tm id cenv tf e le te sp sps bes cs sz m2 b f2 ofs,
-  sp = fresh_block true sps ->
+  sp = fresh_block sps ->
   match_callstack f1 m1 tm
     (Frame (PTree.remove id cenv) tf e le te sp sps bes (Mem.support m1) :: cs)
     (Mem.support m1) (Mem.support tm) ->
-  Mem.alloc true m1 0 sz = (m2, b) ->
+  Mem.alloc m1 0 sz = (m2, b) ->
   cenv!id = Some ofs ->
   inject_incr f1 f2 ->
   f2 b = Some(sp, ofs) ->
@@ -813,7 +813,7 @@ Definition cenv_mem_separated (cenv: compilenv) (vars: list (ident * Z)) (f: mem
 
 Lemma match_callstack_alloc_variables_rec:
   forall tm sp sps tf cenv le te bes cs,
-  sp = fresh_block true sps ->
+  sp = fresh_block sps ->
   Mem.valid_block tm sp ->
   fn_stackspace tf <= Ptrofs.max_unsigned ->
   (forall ofs k p, Mem.perm tm sp ofs k p -> 0 <= ofs < fn_stackspace tf) ->
@@ -874,7 +874,7 @@ Qed.
 
 Lemma match_callstack_alloc_variables:
   forall tm1 sp tm2 m1 vars e m2 cenv f1 cs fn le te,
-  Mem.alloc true tm1 0 (fn_stackspace fn) = (tm2, sp) ->
+  Mem.alloc tm1 0 (fn_stackspace fn) = (tm2, sp) ->
   fn_stackspace fn <= Ptrofs.max_unsigned ->
   alloc_variables empty_env m1 vars e m2 ->
   list_norepet (map fst vars) ->
@@ -1254,7 +1254,7 @@ Theorem match_callstack_function_entry:
   alloc_variables Csharpminor.empty_env m (Csharpminor.fn_vars fn) e m' ->
   bind_parameters (Csharpminor.fn_params fn) args (create_undef_temps fn.(fn_temps)) = Some le ->
   Val.inject_list f args targs ->
-  Mem.alloc true tm 0 tf.(fn_stackspace) = (tm', sp) ->
+  Mem.alloc tm 0 tf.(fn_stackspace) = (tm', sp) ->
   match_callstack f m tm cs (Mem.support m) (Mem.support tm) ->
   Mem.inject f m tm ->
   let te := set_locals (Csharpminor.fn_temps fn) (set_params targs (Csharpminor.fn_params fn)) in
@@ -1600,7 +1600,7 @@ Inductive match_cont: Csharpminor.cont -> Cminor.cont -> compilenv -> exit_env -
   | match_Kcall: forall optid fn e le k tfn sp sps te tk cenv xenv bes es cs sz cenv',
       transl_funbody cenv sz fn = OK tfn ->
       match_cont k tk cenv xenv cs ->
-      sp = fresh_block true sps ->
+      sp = fresh_block sps ->
       match_cont (Csharpminor.Kcall optid fn e le k)
                  (Kcall optid tfn (Vptr sp Ptrofs.zero) te tk)
                  cenv' nil
@@ -1609,7 +1609,7 @@ Inductive match_cont: Csharpminor.cont -> Cminor.cont -> compilenv -> exit_env -
 Inductive match_states: Csharpminor.state -> Cminor.state -> Prop :=
   | match_state:
       forall fn s k e le m tfn ts tk sp sps te tm cenv xenv f bes es cs sz
-      (SPS: sp = fresh_block true sps)
+      (SPS: sp = fresh_block sps)
       (TRF: transl_funbody cenv sz fn = OK tfn)
       (TR: transl_stmt cenv xenv s = OK ts)
       (MINJ: Mem.inject f m tm)
@@ -1621,7 +1621,7 @@ Inductive match_states: Csharpminor.state -> Cminor.state -> Prop :=
                    (State tfn ts tk (Vptr sp Ptrofs.zero) te tm)
   | match_state_seq:
       forall fn s1 s2 k e le m tfn ts1 tk sp sps te tm cenv xenv f bes es cs sz
-      (SPS: sp = fresh_block true sps)
+      (SPS: sp = fresh_block sps)
       (TRF: transl_funbody cenv sz fn = OK tfn)
       (TR: transl_stmt cenv xenv s1 = OK ts1)
       (MINJ: Mem.inject f m tm)
@@ -1815,7 +1815,7 @@ Qed.
 
 Lemma switch_match_states:
   forall fn k e le m tfn ts tk sp sps te tm cenv xenv f bes es cs sz ls body tk'
-    (SPS: sp = fresh_block true sps)
+    (SPS: sp = fresh_block sps)
     (TRF: transl_funbody cenv sz fn = OK tfn)
     (TR: transl_lblstmt cenv (switch_env ls xenv) ls body = OK ts)
     (MINJ: Mem.inject f m tm)
